Add BExp_AppendMask and BExp_Mask

src/tools/angr/bir_angrScript.sml
@@ -1,25 +1,100 @@
 open HolKernel Parse boolLib bossLib;
 
+open HolBACoreSimps
+open bir_expTheory bir_exp_immTheory bir_valuesTheory
+open bir_typing_expTheory bir_envTheory wordsTheory
+open bir_exp_immSyntax
+
 val _ = new_theory "bir_angr";
 
-  val _ = if type_of “BirMask” = Type‘:bir_exp_t -> num -> num -> bir_exp_t’
-          then ()
-          else new_constant ("BirMask",Type‘:bir_exp_t -> num -> num -> bir_exp_t’);
-  val _ = if type_of “BirAppendMask” = Type‘:(bir_exp_t # num # num) list -> bir_exp_t’
-          then ()
-          else new_constant ("BirAppendMask",Type‘:(bir_exp_t # num # num) list -> bir_exp_t’);
+val BExp_Mask_def = Define `
+    BExp_Mask sz u l e =
+      BExp_BinExp BIExp_And
+        (BExp_BinExp BIExp_RightShift e (BExp_Const (n2bs l sz)))
+        (BExp_Const (n2bs (2 ** (u - l + 1) - 1) sz))
+`;
+(*
+EVAL ``BExp_Const (Imm16 (((1w) << (7-0+1))-1w))``
+
+EVAL ``n2bs (2 ** (size_of_bir_immtype Bit8) - (2 ** 1)) Bit8``
+
+EVAL ``n2bs (2 ** (size_of_bir_immtype Bit8) - 1) Bit8``
+
+val test_exp2 = ``(BExp_Const (n2bs 0x731 Bit16))``;
+val test_exp = ``BExp_Mask Bit16 6 3 (BExp_Const (n2bs 0x731 Bit16))``;
+EVAL ``^test_exp``
+
+bir_immTheory.n2bs_def
+EVAL ``type_of_bir_exp ^test_exp``
+(bir_valuesSyntax.dest_BType_Imm o optionSyntax.dest_some o snd o dest_eq o concl o EVAL) ``type_of_bir_exp ^test_exp2``
+
+EVAL ``bir_eval_exp ^test_exp bir_env_empty``
+``0x6``
+*)
   
-  val BirMask_type_of = store_thm ("BirMask_type_of",
- ``!e u l. type_of_bir_exp (BirMask e u l) =
-    type_of_bir_exp e``,
-                    cheat);
- val BirAppendMask_type_of = store_thm ("BirAppendMask_type_of",
- ``!es. type_of_bir_exp (BirAppendMask es) =
- if LENGTH es > 0
- then case bir_immtype_of_size (FOLDR $+ (0:num) (MAP (\ (_,u,l). u-l+1) es)) of
-          NONE => NONE
-         | SOME ty => SOME (BType_Imm ty)
- else NONE``,
-        cheat);
+val BExp_Mask_type_of = store_thm
+  ("BExp_Mask_type_of", ``
+!sz u l e. type_of_bir_exp (BExp_Mask sz u l e) =
+           if (type_of_bir_exp e = SOME (BType_Imm sz)) then
+               SOME (BType_Imm sz) else NONE
+``,
+  REPEAT GEN_TAC >>
+  SIMP_TAC (std_ss++holBACore_ss) [BExp_Mask_def, type_of_bir_exp_def,
+    pairTheory.pair_case_thm] >>
+  REPEAT CASE_TAC >> (
+    FULL_SIMP_TAC (std_ss++holBACore_ss) [bir_type_checker_DEFS]
+  )
+);
+
+
+
+val masklist_size_def = Define `
+    masklist_size l =
+      bir_immtype_of_size (SUM (MAP (\(u,l,_). u-l+1) l))
+`;
+
+val masklist_fold_def = Define `
+    masklist_fold sz (u,l,e) (orbits, ore) =
+      (orbits + u-l+1,
+       BExp_BinExp BIExp_Or
+         (BExp_BinExp BIExp_LeftShift (BExp_Mask sz u l e) (BExp_Const (n2bs orbits sz)))
+         ore)
+`;
+
+val BExp_AppendMask_def = Define `
+    BExp_AppendMask l =
+      if IS_NONE (masklist_size l) then
+        BExp_BinExp BIExp_And (BExp_Const (Imm1 0w)) (BExp_Const (Imm8 0w))
+      else
+        SND (FOLDR (masklist_fold (THE (masklist_size l)))
+                   (0, BExp_Const (n2bs 0 (THE (masklist_size l))))
+                   l)
+`;
+(*
+EVAL ``FOLDR (\x. \a. (x+1)::a) [] [1;2;3]``
+type_of ``masklist_fold``
+type_of ``Bit1``
+
+val test_exp = ``BExp_AppendMask [
+  (10, 3, BExp_Const (n2bs 0xBEEF Bit16));
+  (6, 3, BExp_Const (n2bs 0xBEEF Bit16));
+  (6, 3, BExp_Const (n2bs 0xBEEF Bit16))]``;
+EVAL ``^test_exp``;
+
+EVAL ``bir_eval_exp ^test_exp bir_env_empty``
+``0xDDDD``
+*)
+
+val BExp_AppendMask_type_of = store_thm
+  ("BExp_AppendMask_type_of", ``
+!l. type_of_bir_exp (BExp_AppendMask l) =
+ if LENGTH l > 0
+ then case masklist_size l of
+         NONE => NONE
+       | SOME ty => SOME (BType_Imm ty)
+ else NONE
+``,
+  cheat
+);
 
 val _ = export_theory();
